soundness refined...

Stlc_sound.v
@@ -1,63 +1,15 @@
 From SFL Require Import Imports Auxiliaries Terms Typecheck Eval Progress Preservation.
 Require Import Coq.Strings.String.
 
-Require Import Coq.Relations.Relations.
-
-Inductive multi {X:Type} (R: relation X) : relation X :=
-  | multi_refl : forall (x : X), multi R x x
-  | multi_step : forall (x y z : X),
-                    R x y ->
-                    multi R y z ->
-                    multi R x z.
-
-Definition step (t t': term ): Prop := beta t = Some t'.
-
-Definition multistep := multi step.
-
-Definition normal_form {X : Type} (R : relation X) (t : X) : Prop :=
-  ~ exists t', R t t'.
-
-Definition normal_form_a (e: term) :=
-  let be := beta e in
-  match be with
-    | Some be' => if term_eqb be' e then true else false
-    | _        => false
-  end.
-
-Definition stuck (e: term) :=
-  (normal_form step) e /\ isvalue e = false.
 
 
-Definition stuck_a (e: term) :=
-  normal_form_a e = true /\ isvalue e = false.
+Definition stuck (t: term) := beta t = None /\ isvalue t = false.
 
-
-Definition stuck_b (t: term) := beta t = None /\ isvalue t = false.
-
-Theorem soundness: forall t t' T, 
-  typecheck nil t = Some T /\ 
-  multistep t t' -> 
-  ~ stuck t'.
-Proof. intros t t' T (H, H0). unfold stuck.
-       induction H0; intros.
-       - unfold not. intros (Hnf, Hnv).
-         unfold normal_form in *. apply Hnf.
-         unfold step.
-         specialize (progress x T H); intros.
-         destruct H0. rewrite Hnv in H0. easy.
-         destruct H0. exists x0. easy.
-       - unfold not. intros (Hnf, Hnv).
-         unfold step in *.
-         specialize (preservation x y T (conj H H0)); intros.
-         specialize (IHmulti H2).
-         apply IHmulti. split; easy.
-Qed.
-
-Theorem soundness_R: forall n t t' T, 
+Theorem soundness: forall n t t' T, 
   typecheck nil t = Some T /\
   evaln t n  = Some t' -> 
-  ~ stuck_b t'.
-Proof. unfold stuck_b, not.
+  ~ stuck t'.
+Proof. unfold stuck, not.
        intro n.
        induction n as [| m IHn]; intros t t' T (Ha, Hb) (Hne, Hnv).
        - cbn in Hb. inversion Hb. rewrite <- H0 in *.
@@ -78,39 +30,17 @@ Proof. unfold stuck_b, not.
            apply IHn. split; easy.
 Qed.
 
-Theorem soundness_Q: forall n t T, 
+Theorem soundness_None: forall n t T, 
   typecheck nil t = Some T /\
   evaln t n = None -> 
-  ~ stuck_b t.
-Proof. intros n. unfold stuck_b.
+  ~ stuck t.
+Proof. intros n. unfold stuck.
        induction n; intros t T (H, H0).
        - unfold not. intros (Hnf, Hnv).
          specialize (progress t T H); intros.
          cbn in *. inversion H0.
        - unfold not. intros (Hnf, Hnv).
-         unfold step in *.
          specialize (progress t T H); intros.
          destruct H1. rewrite H1 in Hnv. easy.
          destruct H1. rewrite H1 in Hnf. easy.
 Qed.
-
-
-Theorem soundness_a: forall t t' T, 
-  typecheck nil t = Some T /\ 
-  multistep t t' -> 
-  ~ stuck_b t'.
-Proof. intros t t' T (H, H0). unfold stuck_b.
-       induction H0.
-       - unfold not. intros (Hnf, Hnv).
-         specialize (progress x T H); intros.
-         destruct H0. rewrite H0 in Hnv. easy.
-         destruct H0 as (t, Ha).
-         rewrite Ha in Hnf. easy.
-       - unfold not. intros (Hnf, Hnv).
-         unfold step in *.
-         specialize (preservation x y T (conj H H0)); intros.
-         specialize (IHmulti H2).
-         apply IHmulti. split; easy.
-Qed.
-
-(* Compute beta (App (NVal 5) (BVal false)). *)
